Admitted proof for addAll

skip_list/spec/add.v
@@ -116,5 +116,176 @@ Module AddSpec (Params: SKIP_LIST_PARAMS).
           rewrite Hpred_down; by iExFalso.
     Qed.
 
+    Fixpoint add_key (L: list (gset Z)) (key: Z) : list (gset Z) :=
+      match L with
+      | nil => nil
+      | Stop :: Sbots => (Stop ∪ {[ key ]}) :: (add_key Sbots key)
+      end.
+
+    Theorem addAll_spec (curr top_head: node_rep) (key lvl: Z) (q: frac)
+      (Stop: gset Z) (Sbots: list (gset Z)) 
+      (top: lazy_gname) (bots: list lazy_gname) :
+      INT_MIN < key < INT_MAX →
+      {{{
+        skip_list_equiv top_head lvl q (Stop :: Sbots) (top :: bots)
+        ∗
+        (⌜ curr = top_head ⌝ ∨ own (s_auth top) (◯ {[ curr ]}))
+        ∗
+        ⌜ node_key curr < key ⌝
+      }}}
+        addAll (rep_to_node curr) #key
+      {{{ v new, RET v;
+        (
+          ⌜ v = NONEV ⌝
+          ∗
+          skip_list_equiv top_head lvl q (Stop :: Sbots) (top :: bots)
+        )
+        ∨ 
+        (
+          ⌜ v = SOMEV (rep_to_node new) ⌝
+          ∗ 
+          own (s_auth top) (◯ {[ new ]})
+          ∗ 
+          own (s_toks top) (GSet {[ node_key new ]})
+          ∗ 
+          ⌜ node_key new = key ⌝
+          ∗
+          skip_list_equiv top_head lvl q (add_key (Stop :: Sbots) key) (top :: bots)
+        )
+      }}}.
+    Proof.
+      iIntros (Hkey_range Φ) "(Hlist & Hown_curr & Hrange) HΦ".
+      iRevert (Φ curr top_head lvl Stop Sbots top bots) "Hlist Hown_curr Hrange HΦ".
+      iLöb as "IH".
+      iIntros (Φ curr top_head lvl Stop Sbots top bots) "Hlist #Hown_curr %Hrange HΦ".
+
+      wp_lam. wp_let.
+      iPoseProof (skip_list_equiv_cons with "Hlist") as (P) "(Hinv & Hlist)".
+      wp_apply (find_frac_spec with "[Hinv]").
+      { iFrame "# ∗". iPureIntro; lia. }
+
+      iIntros (pred succ) "(%Hrange' & #Hown_pred & #Hown_succ & _)".
+      wp_pures. wp_lam. wp_pures.
+
+      destruct Sbots as [|Sbot Sbots]; destruct bots as [|bot bots]; try by iExFalso.
+      + iDestruct "Hlist" as "(%Hlvl & Hlazy & %Hnone)".
+        iDestruct "Hlazy" as (Sfrac) "(%Hequiv & Hown_frag & #Hinv)".
+        destruct (node_down pred) as [d|] eqn:Hpred_down; wp_pures.
+        - wp_bind (Load _).
+          iInv (levelN lvl) as (S Skeys L) "(>%Hperm & _ & _ & >Hown_auth & _ & _ & Hlist)" "_".
+
+          iDestruct "Hown_pred" as "[%Heq | #Hown_pred]"; first by congruence.
+          iDestruct (own_valid_2 with "Hown_auth Hown_pred") 
+            as %[Hvalid%gset_included]%auth_both_valid_discrete.
+          rewrite (list_equiv_invert_L L top_head pred); last first.
+          { rewrite Hperm -elem_of_list_In elem_of_elements; set_solver. }
+
+          iDestruct "Hlist" as (? ? ? ? ?) "(_ & _ & _ & _ & _ & >HP & _)".
+          rewrite Hpred_down; by iExFalso.
+        - wp_apply (tryInsert_spec with "[Hown_frag]").
+          { done. }
+          { iFrame "#". iSplit; last (iPureIntro; lia). iExists Sfrac; by iFrame. }
+
+          iIntros (v new) "(Hlazy & Hopt)".
+          iApply "HΦ".
+          iDestruct "Hopt" as "[Hnone | (? & ? & ? & ?)]".
+          * iLeft. iFrame "# ∗".
+            admit.
+          * iRight. by iFrame.          
+      + iDestruct "Hlist" as (l down) "(%Hlvl & Hlazy & %Hsome & Hpt & %Heq_key & Hmatch)".
+        iDestruct "Hlazy" as (Sfrac) "(%Hequiv & Hown_frag & #Hinv)".
+        destruct (node_down pred) as [d|] eqn:Hpred_down; wp_match.
+        - wp_bind (Load _).
+          iInv (levelN lvl) as (S Skeys L) "(>%Hperm & >%Hsort & >%Hequiv' & >Hown_auth & >Hown_frac & >Hown_toks & Hlist)" "Hclose".
+          iDestruct "Hown_pred" as "[%Heq | #Hown_pred]".
+          * assert (d = l) as -> by congruence.
+            wp_load.
+            iMod ("Hclose" with "[Hlist Hown_auth Hown_frac Hown_toks]") as "_".
+            { iNext; iExists S, Skeys, L; by iFrame. }
+
+            iModIntro; wp_pures.
+            wp_apply ("IH" with "[$] [] [%]").
+            { by iLeft. }
+            { rewrite -Heq_key -Heq; lia. }
+
+            iIntros (v new) "Hopt".
+            iDestruct "Hopt" as "[(%Hopt & ?) | (%Hopt & Hown_new & Hown_tok & %Hkey & ?)]".
+            ++ rewrite Hopt. wp_pures.
+               iModIntro. iApply "HΦ".
+               iLeft. iSplit; first done.
+               iFrame "# ∗". iExists l, down. iFrame. 
+               iSplit; first done. iSplit; last done.
+               iExists Sfrac. by iFrame.
+            ++ rewrite Hopt. wp_pures.
+               wp_apply (insert_spec with "[Hown_frag Hown_new Hown_tok]"); auto.
+               { 
+                 iFrame "# ∗".
+                 iSplit; last first.
+                 { iSplit; first by iLeft. iSplit; last done. iPureIntro; lia. }
+                 iExists Sfrac; by iFrame.
+               }
+
+               clear Hkey Hopt new.
+               iIntros (new) "(Hlazy & Hown_new & Hown_tok & %Hkey)".
+               iApply "HΦ". iRight.
+               iFrame. iSplit; first done. iSplit; first done.
+               iExists l, down. by iFrame.
+          * iDestruct (own_valid_2 with "Hown_auth Hown_pred") 
+              as %[Hvalid%gset_included]%auth_both_valid_discrete.
+            rewrite (list_equiv_invert_L L top_head pred); last first.
+            { rewrite Hperm -elem_of_list_In elem_of_elements; set_solver. }
+
+            iDestruct "Hlist" as (succ' ? ? l' ?) "(_ & _ & _ & Hpt' & _ & HP & Himp)".
+            rewrite Hpred_down.
+            iDestruct "HP" as (down') "(Hpt_down & >Hauth_down' & >Htoks_down' & >%Hdown'_key)".
+
+            assert ({[ down' ]} = {[ down' ]} ⋅ {[ down' ]}) as -> by set_solver.
+            iDestruct "Hauth_down'" as "(Hauth_down' & Hauth_down'_dup)".
+
+            wp_load.
+            iPoseProof ("Himp" with "[Hpt' Hpt_down Hauth_down' Htoks_down']") as "Hlist".
+            { iFrame; iExists down'; by iFrame. }
+            iMod ("Hclose" with "[Hlist Hown_auth Hown_frac Hown_toks]") as "_".
+            { iNext; iExists S, Skeys, L; by iFrame. }
+
+            iModIntro; wp_pures.
+            wp_apply ("IH" with "[$] [$] [%]").
+            { lia. }
+
+            iIntros (v new) "Hopt".
+            iDestruct "Hopt" as "[(%Hopt & ?) | (%Hopt & Hown_new & Hown_tok & %Hkey & ?)]".
+            ++ rewrite Hopt. wp_pures.
+               iModIntro. iApply "HΦ".
+               iLeft. iSplit; first done.
+               iFrame "# ∗". iExists l, down. iFrame. 
+               iSplit; first done. iSplit; last done.
+               iExists Sfrac. by iFrame.
+            ++ rewrite Hopt. wp_pures.
+               wp_apply (insert_spec with "[Hown_frag Hown_new Hown_tok]"); auto.
+               { 
+                 iFrame "# ∗".
+                 iSplit; last first.
+                 { iSplit; last done. iPureIntro; lia. }
+                 iExists Sfrac; by iFrame.
+               }
+
+               clear Hkey Hopt new.
+               iIntros (new) "(Hlazy & Hown_new & Hown_tok & %Hkey)".
+               iApply "HΦ". iRight.
+               iFrame. iSplit; first done. iSplit; first done.
+               iExists l, down. by iFrame.
+        - iAssert (|={⊤}=> False)%I as "Hfalse"; last by iMod "Hfalse".
+          iInv (levelN lvl) as (S Skeys L) "(>%Hperm & _ & _ & >Hown_auth & _ & _ & Hlist)" "_".
+        
+          iDestruct "Hown_pred" as "[%Heq | #Hown_pred]"; first by congruence.
+          iDestruct (own_valid_2 with "Hown_auth Hown_pred") 
+            as %[Hvalid%gset_included]%auth_both_valid_discrete.
+          rewrite (list_equiv_invert_L L top_head pred); last first.
+          { rewrite Hperm -elem_of_list_In elem_of_elements; set_solver. }
+
+          iDestruct "Hlist" as (? ? ? ? ?) "(_ & _ & _ & _ & _ & >HP & _)".
+          by rewrite Hpred_down.
+    Admitted.
+
   End Proofs.
 End AddSpec.
